Add physical actions to reactors

src/ReactorModel/Execution/Reactor.lean
@@ -10,10 +10,11 @@ variable [Indexable α] in section
 def dependencies (rtr : α) (rcn : ID) : Set ID := 
   { rcn' | rcn' <[rtr] rcn }
 
-structure Refresh (rtr₁ rtr₂ : α) (acts : ID ⇀ Value) : Prop where
+structure Refresh (rtr₁ rtr₂ : α) (logs : ID ⇀ Value) : Prop where
   equiv    : rtr₁ ≈ rtr₂
-  eq_state : rtr₂[.stv] = rtr₁[.stv]
-  acts     : rtr₂[.act] = acts
+  state    : rtr₂[.stv] = rtr₁[.stv]
+  logs     : rtr₂[.log] = logs
+  phys     : rtr₂[.phy] = rtr₁[.phy].map fun _ => .absent
   inputs   : rtr₂[.inp] = rtr₁[.inp].map fun _ => .absent
   outputs  : rtr₂[.out] = rtr₁[.out].map fun _ => .absent
 
@@ -21,9 +22,10 @@ end
 
 variable [Proper α] [Finite α]
 
-def refresh (rtr : α) (acts : ID ⇀ Value) : α :=
+def refresh (rtr : α) (logs : ID ⇀ Value) : α :=
   let rtr₁ := set rtr  .inp $ Partial.const (rtr[.inp].ids : Set ID) .absent
   let rtr₂ := set rtr₁ .out $ Partial.const (rtr[.out].ids : Set ID) .absent
-  set rtr₂ .act acts
+  let rtr₃ := set rtr₂ .phy $ Partial.const (rtr[.phy].ids : Set ID) .absent
+  set rtr₃ .log logs
 
 end Reactor
