src/ReactorModel/Objects/Component.lean
@@ -1,11 +1,15 @@
 import ReactorModel.Primitives
 
-inductive Component.Valued
+inductive Component.Writable
   | inp -- Input port
   | out -- Output port
   | stv -- State variable
-  | act -- Action
-  
+  | log -- Logical action
+
+inductive Component.Valued
+  | wrt (s : Component.Writable)
+  | phy -- Physical action
+
 -- An enumeration of the different *kinds* of components that are addressable by ids in a reactor.
 inductive Component
   | val (v : Component.Valued)
@@ -14,12 +18,21 @@ inductive Component
 
 namespace Component
 
+@[match_pattern] abbrev Valued.inp := Valued.wrt .inp
+@[match_pattern] abbrev Valued.out := Valued.wrt .out
+@[match_pattern] abbrev Valued.stv := Valued.wrt .stv
+@[match_pattern] abbrev Valued.log := Valued.wrt .log
+
 @[match_pattern] abbrev inp := Component.val .inp
 @[match_pattern] abbrev out := Component.val .out
-@[match_pattern] abbrev act := Component.val .act
 @[match_pattern] abbrev stv := Component.val .stv
+@[match_pattern] abbrev log := Component.val .log
+@[match_pattern] abbrev phy := Component.val .phy
 
-instance : Coe Component.Valued Component where
+instance : Coe Writable Valued where
+  coe := Valued.wrt 
+
+instance : Coe Valued Component where
   coe := val 
 
 -- The type of `WithTop ID`s extends the type of `ID`s with a `⊤` ID witch is used to refer to a/the
