src/ReactorModel/Execution/Theorems/Reactor.lean
@@ -33,33 +33,42 @@ theorem Refresh.deterministic {rtr : α} (rf₁ : Refresh rtr rtr₁ as) (rf₂ 
   have e := Equivalent.trans (Equivalent.symm rf₁.equiv) rf₂.equiv
   apply ext_obj? e
   intro cpt _ _ _ ho₁ ho₂
-  cases cpt
-  case stv => injection (rf₁.eq_state ▸ ho₁) ▸ rf₂.eq_state ▸ ho₂
-  case act => injection (rf₁.acts     ▸ ho₁) ▸ rf₂.acts     ▸ ho₂
-  case inp => injection (rf₁.inputs   ▸ ho₁) ▸ rf₂.inputs   ▸ ho₂
-  case out => injection (rf₁.outputs  ▸ ho₁) ▸ rf₂.outputs  ▸ ho₂
+  cases cpt <;> try cases ‹Component.Writable›
+  case stv => injection (rf₁.state   ▸ ho₁) ▸ rf₂.state   ▸ ho₂
+  case log => injection (rf₁.logs    ▸ ho₁) ▸ rf₂.logs    ▸ ho₂
+  case phy => injection (rf₁.phys    ▸ ho₁) ▸ rf₂.phys    ▸ ho₂
+  case inp => injection (rf₁.inputs  ▸ ho₁) ▸ rf₂.inputs  ▸ ho₂
+  case out => injection (rf₁.outputs ▸ ho₁) ▸ rf₂.outputs ▸ ho₂
 
 variable [Finite α]
 
-theorem refresh_correct (rtr : α) (h : acts.ids = rtr[.act].ids) : 
-    Refresh rtr (refresh rtr acts) acts where
-  equiv := Equivalent.trans set_equiv $ Equivalent.trans set_equiv set_equiv
-  eq_state := by
+open Equivalent in
+theorem refresh_correct (rtr : α) (h : logs.ids = rtr[.log].ids) : 
+    Refresh rtr (refresh rtr logs) logs where
+  equiv := trans set_equiv $ trans set_equiv $ trans set_equiv set_equiv
+  state := by
     rw [
-      refresh, set_preserves (by simp : .stv ≠ .act), set_preserves (by simp : .stv ≠ .out), 
-      set_preserves (by simp : .stv ≠ .inp)
+      refresh, set_preserves (by simp : .stv ≠ .log), set_preserves (by simp : .stv ≠ .phy), 
+      set_preserves (by simp : .stv ≠ .out), set_preserves (by simp : .stv ≠ .inp)
     ]
-  acts := by 
-    rw [refresh, set_updated $ h ▸ (Equivalent.ids_eq $ Equivalent.trans set_equiv set_equiv)]
+  logs := by 
+    rw [refresh, set_updated $ h ▸ (ids_eq $ trans set_equiv $ trans set_equiv set_equiv)]
+  phys := by 
+    rw [
+      refresh, set_preserves (by simp : .phy ≠ .log),
+      set_updated $ by rw [ids_eq $ Equivalent.trans set_equiv set_equiv, Partial.const_ids _ _], 
+      Partial.const_eq_map_const
+    ]
   inputs := by 
     rw [
-      refresh, set_preserves (by simp : .inp ≠ .act), set_preserves (by simp : .inp ≠ .out), 
-      set_updated $ Partial.const_ids _ _, Partial.const_eq_map_const
+      refresh, set_preserves (by simp : .inp ≠ .log), set_preserves (by simp : .inp ≠ .phy), 
+      set_preserves (by simp : .inp ≠ .out), set_updated $ Partial.const_ids _ _, 
+      Partial.const_eq_map_const
     ]
   outputs := by 
     rw [
-      refresh, set_preserves (by simp : .out ≠ .act),
-      set_updated $ by rw [Equivalent.ids_eq set_equiv, Partial.const_ids _ _],
+      refresh, set_preserves (by simp : .out ≠ .log), set_preserves (by simp : .out ≠ .phy), 
+      set_updated $ by rw [ids_eq set_equiv, Partial.const_ids _ _],
       Partial.const_eq_map_const
     ]
 
